Test.thy
@@ -2,6 +2,7 @@ theory Test
   imports Demo_Hoare
 begin
 
+
 lemma True
 proof 
 
@@ -15,12 +16,11 @@ proof
 (* TODO: should be handled by program-command *)
   define prog where "prog = [Set STR ''x'' 5, Guess STR ''y'', Add STR ''x'' STR ''y'']"
 
-(* TODO: should be handled by program-command *)
-  do \<open>snd o add_invariant \<^binding>\<open>start\<close> \<^term>\<open>(\<lambda>m::mem. True)\<close>\<close>
+  invariant (demo_logic) start: "\<lambda>m. True"
 
   (* Step 1: Set x 5 *)
 
-  do_prf \<open>add_hoare3 \<^binding>\<open>step1\<close> NONE (Demo_Hoare_Logic.ex_range (0,1)) "start"
+  do_prf \<open>Forward_Hoare.add_hoare3 \<^binding>\<open>step1\<close> NONE (Demo_Hoare.ex_range (0,1)) "start"
      \<^term>\<open>(postcondition_trivial (Set STR ''x'' 5) start_inv)\<close>\<close>
     using step1_inv_def step1_prog_def by (rule valid)
 
@@ -29,14 +29,14 @@ proof
 
   (* Step 2: Guess y *)
 
-  do_prf \<open>add_hoare3 \<^binding>\<open>step2\<close> NONE (Demo_Hoare_Logic.ex_range (1,2)) "step1"
+  do_prf \<open>Forward_Hoare.add_hoare3 \<^binding>\<open>step2\<close> NONE (Demo_Hoare.ex_range (1,2)) "step1"
     \<^term>\<open>postcondition_pick (Guess STR ''y'') (-5) step1_inv\<close>\<close>
     using step2_inv_def step2_prog_def by (rule valid)
 
   have step2_x5: "pc_imp step2_inv (\<lambda>m. m STR ''x'' = 5)"
     using step2_inv_def apply (rule unchanged)
      apply (rule independent_ofI, simp)
-    apply (tactic \<open>use_facts_tac \<^context> @{thms step1_x5} 1\<close>)
+    apply (tactic \<open>Demo_Hoare.use_facts_tac \<^context> @{thms step1_x5} 1\<close>)
     by simp
 
   have step2_y5: "pc_imp step2_inv (\<lambda>m. m STR ''y'' = -5)"
@@ -47,7 +47,7 @@ proof
 
   (* Step 3: Add x y *)
 
-  do_prf \<open>add_hoare3 \<^binding>\<open>step3\<close> NONE (Demo_Hoare_Logic.ex_range (2,3)) "step2"
+  do_prf \<open>Forward_Hoare.add_hoare3 \<^binding>\<open>step3\<close> NONE (Demo_Hoare.ex_range (2,3)) "step2"
     \<^term>\<open>(postcondition_trivial (Add STR ''x'' STR ''y'') step2_inv)\<close>\<close>
     using step3_inv_def step3_prog_def by (rule valid, simp)
 
@@ -55,13 +55,13 @@ proof
     using step3_inv_def apply (rule unchanged)
       apply (rule independent_ofI, simp)
      apply simp
-    apply (tactic \<open>use_facts_tac \<^context> @{thms step2_y5} 1\<close>)
+    apply (tactic \<open>Demo_Hoare.use_facts_tac \<^context> @{thms step2_y5} 1\<close>)
     by simp
 
   have step3_x0: "pc_imp step3_inv (\<lambda>m. m STR ''x'' = 0)"
     using step3_inv_def apply (rule wp)
      apply simp
-    apply (tactic \<open>use_facts_tac \<^context> @{thms step2_x5 step2_y5} 1\<close>)
+    apply (tactic \<open>Demo_Hoare.use_facts_tac \<^context> @{thms step2_x5 step2_y5} 1\<close>)
     by simp
 
   have start_step3: "hoare start_inv prog step3_inv"
